{
 "cells": [
  {
   "cell_type": "markdown",
   "id": "54efa185-94c4-48c9-9159-0c1084e8f38b",
   "metadata": {},
   "source": [
    "ques1. Find the value of T(2) for the recurrence relation T(n) = 3T(n-1) + 12n, given that T(0)=5."
   ]
  },
  {
   "cell_type": "markdown",
   "id": "070fa224-71e5-4e68-878a-8a3a63694505",
   "metadata": {},
   "source": [
    "To find the value of \\( T(2) \\) for the recurrence relation \\( T(n) = 3T(n-1) + 12n \\) with \\( T(0) = 5 \\), we will compute \\( T(n) \\) step-by-step using the given recurrence relation.\n",
    "\n",
    "### Step-by-Step Calculation\n",
    "\n",
    "1. **Compute \\( T(1) \\):**\n",
    "\n",
    "   Given:\n",
    "   \\[\n",
    "   T(n) = 3T(n-1) + 12n\n",
    "   \\]\n",
    "   Substitute \\( n = 1 \\):\n",
    "   \\[\n",
    "   T(1) = 3T(0) + 12 \\cdot 1\n",
    "   \\]\n",
    "   We know \\( T(0) = 5 \\):\n",
    "   \\[\n",
    "   T(1) = 3 \\cdot 5 + 12 \\cdot 1\n",
    "   \\]\n",
    "   \\[\n",
    "   T(1) = 15 + 12\n",
    "   \\]\n",
    "   \\[\n",
    "   T(1) = 27\n",
    "   \\]\n",
    "\n",
    "2. **Compute \\( T(2) \\):**\n",
    "\n",
    "   Substitute \\( n = 2 \\) into the recurrence relation:\n",
    "   \\[\n",
    "   T(2) = 3T(1) + 12 \\cdot 2\n",
    "   \\]\n",
    "   We found \\( T(1) = 27 \\):\n",
    "   \\[\n",
    "   T(2) = 3 \\cdot 27 + 12 \\cdot 2\n",
    "   \\]\n",
    "   \\[\n",
    "   T(2) = 81 + 24\n",
    "   \\]\n",
    "   \\[\n",
    "   T(2) = 105\n",
    "   \\]\n",
    "\n",
    "### Conclusion\n",
    "\n",
    "The value of t(2) is 105"
   ]
  },
  {
   "cell_type": "code",
   "execution_count": null,
   "id": "b5eea95c-fed5-4083-90e5-cc2244481fea",
   "metadata": {},
   "outputs": [],
   "source": []
  },
  {
   "cell_type": "markdown",
   "id": "9634b8da-c9fe-4082-853a-70a560b31a7a",
   "metadata": {},
   "source": [
    "ques2. Given a rec%rrence relation, solve it %sing the s%bstit%tion method:\n",
    "\n",
    "a. T(n) = T(n-1) + c\n",
    "\n",
    "b. T(n) = 2T(n/2) + n\n",
    "\n",
    "c. T(n) = 2T(n/2) + c\n",
    "\n",
    "d. T(n) = T(n/2) + c"
   ]
  },
  {
   "cell_type": "markdown",
   "id": "a20e53fe-7b69-48a5-8b31-502791162573",
   "metadata": {},
   "source": [
    "To solve recurrence relations using the substitution method, we'll assume a solution form and then use induction to verify it. Let's tackle each recurrence relation one by one.\n",
    "\n",
    "### a. \\( T(n) = T(n-1) + c \\)\n",
    "\n",
    "**1. Assume a solution form:**\n",
    "\n",
    "Assume \\( T(n) = an + b \\), where \\( a \\) and \\( b \\) are constants to be determined.\n",
    "\n",
    "**2. Substitute into the recurrence relation:**\n",
    "\n",
    "Substitute \\( T(n) = an + b \\) into \\( T(n) = T(n-1) + c \\):\n",
    "\\[\n",
    "T(n) = a(n-1) + b + c\n",
    "\\]\n",
    "\\[\n",
    "T(n) = an - a + b + c\n",
    "\\]\n",
    "\n",
    "For this to match \\( T(n) = an + b \\), we must have:\n",
    "\\[\n",
    "-an + a + b + c = b\n",
    "\\]\n",
    "\\[\n",
    "-a + c = 0 \\implies a = c\n",
    "\\]\n",
    "\n",
    "Thus, the solution is:\n",
    "\\[\n",
    "T(n) = cn + b\n",
    "\\]\n",
    "\n",
    "**3. Determine \\( b \\) using initial conditions:**\n",
    "\n",
    "If \\( T(0) = T_0 \\), then:\n",
    "\\[\n",
    "T(0) = c \\cdot 0 + b \\implies b = T_0\n",
    "\\]\n",
    "\n",
    "So the solution is:\n",
    "\\[\n",
    "T(n) = cn + T_0\n",
    "\\]\n",
    "\n",
    "### b. \\( T(n) = 2T(n/2) + n \\)\n",
    "\n",
    "**1. Assume a solution form:**\n",
    "\n",
    "Assume \\( T(n) = an \\log n + b \\), where \\( a \\) and \\( b \\) are constants to be determined.\n",
    "\n",
    "**2. Substitute into the recurrence relation:**\n",
    "\n",
    "Substitute \\( T(n) = an \\log n + b \\) into \\( T(n) = 2T(n/2) + n \\):\n",
    "\\[\n",
    "T(n) = 2[a(n/2) \\log (n/2) + b] + n\n",
    "\\]\n",
    "\\[\n",
    "T(n) = 2\\left[a(n/2) \\log n - a(n/2) \\log 2 + b\\right] + n\n",
    "\\]\n",
    "\\[\n",
    "T(n) = an \\log n - a n + 2b + n\n",
    "\\]\n",
    "\\[\n",
    "T(n) = an \\log n + (n - a n + 2b)\n",
    "\\]\n",
    "\n",
    "For this to match \\( T(n) = an \\log n + b \\), we need:\n",
    "\\[\n",
    "-n + a n = 0 \\implies a = 1\n",
    "\\]\n",
    "\\[\n",
    "2b = b \\implies b = 2b\n",
    "\\]\n",
    "\n",
    "Thus, the solution is:\n",
    "\\[\n",
    "T(n) = n \\log n + O(n)\n",
    "\\]\n",
    "\n",
    "**In Big-O notation, the solution is \\( T(n) = O(n \\log n) \\).**\n",
    "\n",
    "### c. \\( T(n) = 2T(n/2) + c \\)\n",
    "\n",
    "**1. Assume a solution form:**\n",
    "\n",
    "Assume \\( T(n) = a n + b \\), where \\( a \\) and \\( b \\) are constants to be determined.\n",
    "\n",
    "**2. Substitute into the recurrence relation:**\n",
    "\n",
    "Substitute \\( T(n) = a n + b \\) into \\( T(n) = 2T(n/2) + c \\):\n",
    "\\[\n",
    "T(n) = 2[a(n/2) + b] + c\n",
    "\\]\n",
    "\\[\n",
    "T(n) = an + 2b + c\n",
    "\\]\n",
    "\n",
    "For this to match \\( T(n) = an + b \\), we must have:\n",
    "\\[\n",
    "2b + c = b \\implies b = -c\n",
    "\\]\n",
    "\n",
    "Thus, the solution is:\n",
    "\\[\n",
    "T(n) = a n - c\n",
    "\\]\n",
    "\n",
    "**Since \\( a = c \\), the solution is:**\n",
    "\\[\n",
    "T(n) = c n - c\n",
    "\\]\n",
    "\n",
    "**In Big-O notation, the solution is \\( T(n) = O(n) \\).**\n",
    "\n",
    "### d. \\( T(n) = T(n/2) + c \\)\n",
    "\n",
    "**1. Assume a solution form:**\n",
    "\n",
    "Assume \\( T(n) = a \\log n + b \\), where \\( a \\) and \\( b \\) are constants to be determined.\n",
    "\n",
    "**2. Substitute into the recurrence relation:**\n",
    "\n",
    "Substitute \\( T(n) = a \\log n + b \\) into \\( T(n) = T(n/2) + c \\):\n",
    "\\[\n",
    "T(n) = a \\log (n/2) + b + c\n",
    "\\]\n",
    "\\[\n",
    "T(n) = a (\\log n - \\log 2) + b + c\n",
    "\\]\n",
    "\\[\n",
    "T(n) = a \\log n - a \\log 2 + b + c\n",
    "\\]\n",
    "\n",
    "For this to match \\( T(n) = a \\log n + b \\), we need:\n",
    "\\[\n",
    "-a \\log 2 + c = 0 \\implies a = c\n",
    "\\]\n",
    "\n",
    "Thus, the solution is:\n",
    "\\[\n",
    "T(n) = c \\log n + b - c \\log 2\n",
    "\\]\n",
    "\n",
    "**In Big-O notation, the solution is \\( T(n) = O(\\log n) \\).**\n",
    "\n",
    "### Summary of Solutions:\n",
    "- **a.** \\( T(n) = cn + T_0 \\)\n",
    "- **b.** \\( T(n) = O(n \\log n) \\)\n",
    "- **c.** \\( T(n) = O(n) \\)\n",
    "- **d.** \\( T(n) = O(\\log n) \\)"
   ]
  },
  {
   "cell_type": "code",
   "execution_count": null,
   "id": "7a36f633-5cfb-4ead-8857-c0dbc8cc7531",
   "metadata": {},
   "outputs": [],
   "source": []
  },
  {
   "cell_type": "markdown",
   "id": "74b1d3fd-0f11-4675-9abb-4d63f40c06a8",
   "metadata": {},
   "source": [
    "\n",
    "\n",
    "\n",
    "\n",
    "ques3. Given a rec%rrence relation, solve it %sing the rec%rsive tree approach:\n",
    "a. T(n) = 2T(n-1) +1\n",
    "b. T(n) = 2T(n/2) + n\n",
    "\n"
   ]
  },
  {
   "cell_type": "markdown",
   "id": "9ae78624-8192-4a32-8d76-a64c039eb771",
   "metadata": {},
   "source": [
    "To solve recurrence relations using the recursive tree approach, we break down the problem into a tree structure where each node represents a subproblem. We then sum up the costs at each level of the tree to get the total cost of the problem. Let's tackle each recurrence relation using this approach.\n",
    "\n",
    "### a. \\( T(n) = 2T(n-1) + 1 \\)\n",
    "\n",
    "**1. ** Draw the Recursive Tree:**\n",
    "\n",
    "- **Level 0 (Root):** The root of the tree is \\( T(n) \\).\n",
    "  \\[\n",
    "  T(n)\n",
    "  \\]\n",
    "\n",
    "- **Level 1:** The root splits into two subproblems:\n",
    "  \\[\n",
    "  2T(n-1) + 1\n",
    "  \\]\n",
    "\n",
    "- **Level 2:** Each of the two subproblems from Level 1 further splits into two:\n",
    "  \\[\n",
    "  4T(n-2) + 2 \\cdot 1 = 4T(n-2) + 2\n",
    "  \\]\n",
    "\n",
    "- **Level 3:** Each of the four subproblems from Level 2 further splits into two:\n",
    "  \\[\n",
    "  8T(n-3) + 4 \\cdot 1 = 8T(n-3) + 4\n",
    "  \\]\n",
    "\n",
    "**2. ** Determine the Number of Nodes and Cost at Each Level:**\n",
    "\n",
    "- **Number of Nodes at Level \\( i \\):** \\( 2^i \\)\n",
    "- **Cost at Each Node at Level \\( i \\):** Each node incurs a cost of 1 at that level.\n",
    "  \n",
    "  So, the total cost at level \\( i \\) is:\n",
    "  \\[\n",
    "  \\text{Cost at level } i = 2^i \\cdot 1 = 2^i\n",
    "  \\]\n",
    "\n",
    "**3. ** Determine the Number of Levels:**\n",
    "\n",
    "- The recursion stops when \\( n - i = 0 \\), so the number of levels \\( i \\) is \\( n \\).\n",
    "\n",
    "**4. ** Sum Up the Costs Across All Levels:**\n",
    "\n",
    "The total cost \\( T(n) \\) is the sum of costs at all levels:\n",
    "\\[\n",
    "T(n) = \\sum_{i=0}^{n-1} 2^i\n",
    "\\]\n",
    "This is a geometric series sum:\n",
    "\\[\n",
    "T(n) = 2^n - 1\n",
    "\\]\n",
    "\n",
    "**5. ** Final Solution:**\n",
    "\n",
    "The recurrence relation \\( T(n) = 2T(n-1) + 1 \\) solves to:\n",
    "\\[\n",
    "T(n) = 2^n - 1\n",
    "\\]\n",
    "\n",
    "### b. \\( T(n) = 2T(n/2) + n \\)\n",
    "\n",
    "**1. ** Draw the Recursive Tree:**\n",
    "\n",
    "- **Level 0 (Root):** The root of the tree is \\( T(n) \\).\n",
    "  \\[\n",
    "  T(n)\n",
    "  \\]\n",
    "\n",
    "- **Level 1:** The root splits into two subproblems:\n",
    "  \\[\n",
    "  2T(n/2) + n\n",
    "  \\]\n",
    "\n",
    "- **Level 2:** Each of the two subproblems splits into two more subproblems:\n",
    "  \\[\n",
    "  4T(n/4) + 2 \\cdot (n/2) = 4T(n/4) + n\n",
    "  \\]\n",
    "\n",
    "- **Level 3:** Each of the four subproblems splits into two:\n",
    "  \\[\n",
    "  8T(n/8) + 4 \\cdot (n/4) = 8T(n/8) + n\n",
    "  \\]\n",
    "\n",
    "**2. ** Determine the Number of Nodes and Cost at Each Level:**\n",
    "\n",
    "- **Number of Nodes at Level \\( i \\):** \\( 2^i \\)\n",
    "- **Cost at Each Node at Level \\( i \\):** Each node incurs a cost of \\( n / 2^i \\) at that level.\n",
    "  \n",
    "  So, the total cost at level \\( i \\) is:\n",
    "  \\[\n",
    "  \\text{Cost at level } i = 2^i \\cdot \\frac{n}{2^i} = n\n",
    "  \\]\n",
    "\n",
    "**3. ** Determine the Number of Levels:**\n",
    "\n",
    "- The recursion stops when \\( n / 2^i = 1 \\), so the number of levels \\( i \\) is \\( \\log_2(n) \\).\n",
    "\n",
    "**4. ** Sum Up the Costs Across All Levels:**\n",
    "\n",
    "The total cost \\( T(n) \\) is the sum of costs at all levels:\n",
    "\\[\n",
    "T(n) = \\sum_{i=0}^{\\log_2(n)} n\n",
    "\\]\n",
    "There are \\( \\log_2(n) + 1 \\) levels, each contributing \\( n \\):\n",
    "\\[\n",
    "T(n) = (\\log_2(n) + 1) \\cdot n\n",
    "\\]\n",
    "\\[\n",
    "T(n) = n \\log_2(n) + n\n",
    "\\]\n",
    "\n",
    "**5. ** Final Solution:**\n",
    "\n",
    "The recurrence relation \\( T(n) = 2T(n/2) + n \\) solves to:\n",
    "\\[\n",
    "T(n) = O(n \\log n)\n",
    "\\]\n",
    "\n",
    "### Summary of Solutions:\n",
    "- **a.** \\( T(n) = 2^n - 1 \\)\n",
    "- **b.** \\( T(n) = O(n \\log n) \\)"
   ]
  },
  {
   "cell_type": "code",
   "execution_count": null,
   "id": "5c0783b0-65e1-4661-93f4-8812268ae5f1",
   "metadata": {},
   "outputs": [],
   "source": []
  }
 ],
 "metadata": {
  "kernelspec": {
   "display_name": "Python 3 (ipykernel)",
   "language": "python",
   "name": "python3"
  },
  "language_info": {
   "codemirror_mode": {
    "name": "ipython",
    "version": 3
   },
   "file_extension": ".py",
   "mimetype": "text/x-python",
   "name": "python",
   "nbconvert_exporter": "python",
   "pygments_lexer": "ipython3",
   "version": "3.10.8"
  }
 },
 "nbformat": 4,
 "nbformat_minor": 5
}
